Verificación

Verification/VerificationCDPC.dfy
@@ -15,67 +15,69 @@ method verifyCDPC(f:Map_Map_T<int, bool, bool>, g:Map_Map_T<int, bool, int>, P:S
   requires 0.0 <= a <= b <= 1.0
   requires 0.0 <= x <= y <= 1.0
   ensures r == certificateCDPC(f.Model(), g.Model(), P.Model(), a, b, x, y, iv.Model())
-  {
-    counter := counter_in;
-    var isEmpty:bool; isEmpty, counter := iv.Empty(counter);
-    if (isEmpty) {
-      var nCandidates:int; nCandidates, counter := f.nPairs(counter);
-      if (nCandidates == 0) {
-        return true, counter;
-      }
-      else {
-        var okApt:bool; okApt, counter := correct_apt_ratio(f, x, y, counter);
-        var okPrivate:bool; okPrivate, counter := correct_private_ratio(f, P, a, b, counter);
-        return okApt && okPrivate, counter;
-      }
+{
+  counter := counter_in;
+  var isEmpty:bool; isEmpty, counter := iv.Empty(counter);
+  if (isEmpty) {
+    var nCandidates:int; nCandidates, counter := f.nPairs(counter);
+    if (nCandidates == 0) {
+      return true, counter;
     }
     else {
-      var question:int; question, counter := iv.Key(counter);
-      var f':Map_Map_T<int, bool, bool>; f', counter := f.Copy(counter);
-      var f'Empty:bool; f'Empty, counter := f'.Empty(counter);
-      var ok:bool := true;
-
-      while (!f'Empty)
-        decreases f'.Cardinality()
-        invariant in_universe_Map_Map_T(f', f)
-        invariant ok == (forall cand:candidate | cand in (f.Keys() - f'.Keys()) :: question in cand.Keys)
-      {
-        f', ok, counter := loop_check_that_candidates_have_question(f, f', question, ok, counter);
-      }
-
-      var f_true:Map_Map_T<int, bool, bool>; f_true, counter := candidates_with_same_answer(f, question, true, counter);
-      var f_false:Map_Map_T<int, bool, bool>; f_false, counter := candidates_with_same_answer(f, question, false, counter);
-      var g_true:Map_Map_T<int, bool, int>; g_true, counter := candidates_with_same_answer(g, question, true, counter);
-      var g_false:Map_Map_T<int, bool, int>; g_false, counter := candidates_with_same_answer(g, question, false, counter);
-      
-      var iv_true:Interview; iv_true, counter := iv.Get(true, counter);
-      var iv_false:Interview; iv_false, counter := iv.Get(false, counter);
-
-      var b_true:bool; b_true, counter := verifyCDPC(f_true, g_true, P, a, b, x, y, iv_true, counter);
-      var b_false:bool; b_false, counter := verifyCDPC(f_false, g_false, P, a, b, x, y, iv_false, counter);
-      ok := ok && b_true && b_false;
-
-      return ok, counter;
+      var okApt:bool; okApt, counter := correct_apt_ratio(f, x, y, counter);
+      var okPrivate:bool; okPrivate, counter := correct_private_ratio(f, P, a, b, counter);
+      return okApt && okPrivate, counter;
     }
   }
+  else {
+    var question:int; question, counter := iv.Key(counter);
+    var f':Map_Map_T<int, bool, bool>; f', counter := f.Copy(counter);
+    var f'Empty:bool; f'Empty, counter := f'.Empty(counter);
+    var ok:bool := true;
+
+    while (!f'Empty)
+      decreases f'.Cardinality()
+      invariant in_universe_Map_Map_T(f', f)
+      invariant ok == (forall cand:candidate | cand in (f.Keys() - f'.Keys()) :: question in cand.Keys)
+    {
+      f', ok, counter := loop_check_that_candidates_have_question(f, f', question, ok, counter);
+    }
+
+    var f_true:Map_Map_T<int, bool, bool>; f_true, counter := candidates_with_same_answer(f, question, true, counter);
+    var f_false:Map_Map_T<int, bool, bool>; f_false, counter := candidates_with_same_answer(f, question, false, counter);
+    var g_true:Map_Map_T<int, bool, int>; g_true, counter := candidates_with_same_answer(g, question, true, counter);
+    var g_false:Map_Map_T<int, bool, int>; g_false, counter := candidates_with_same_answer(g, question, false, counter);
+    
+    var iv_true:Interview; iv_true, counter := iv.Get(true, counter);
+    var iv_false:Interview; iv_false, counter := iv.Get(false, counter);
+
+    var b_true:bool; b_true, counter := verifyCDPC(f_true, g_true, P, a, b, x, y, iv_true, counter);
+    var b_false:bool; b_false, counter := verifyCDPC(f_false, g_false, P, a, b, x, y, iv_false, counter);
+    ok := ok && b_true && b_false;
+
+    return ok, counter;
+  }
+}
 
 
-method loop_check_that_candidates_have_question(f:Map_Map_T<int, bool, bool>, f':Map_Map_T<int, bool, bool>, question:int, ok:bool, ghost counter_in:nat) returns (f'':Map_Map_T<int, bool, bool>, ok':bool, ghost counter:nat)
+
+method loop_check_that_candidates_have_question(f:Map_Map_T<int, bool, bool>, f':Map_Map_T<int, bool, bool>, question:int, ok:bool, ghost counter_in:nat) returns (f'_out:Map_Map_T<int, bool, bool>, ok_out:bool, ghost counter:nat)
   requires in_universe_Map_Map_T(f', f)
   requires ok == (forall cand:candidate | cand in (f.Keys() - f'.Keys()) :: question in cand.Keys)
-  ensures in_universe_Map_Map_T(f'', f)
-  ensures ok' == (forall cand:candidate | cand in (f.Keys() - f''.Keys()) :: question in cand.Keys)
-  ensures f''.Cardinality() == f'.Cardinality() - 1
+  ensures in_universe_Map_Map_T(f'_out, f)
+  ensures ok_out == (forall cand:candidate | cand in (f.Keys() - f'_out.Keys()) :: question in cand.Keys)
+  ensures f'_out.Cardinality() == f'.Cardinality() - 1
 {
   counter := counter_in;
   var cand:Map<int, bool>; cand, counter := f'.PickKey(counter);
-  f'', counter := f'.Remove(cand, counter);
+  f'_out, counter := f'.Remove(cand, counter);
   
   var candHasQuestion:bool; candHasQuestion, counter := cand.ContainsKey(question, counter);
-  ok' := ok && candHasQuestion;
+  ok_out := ok && candHasQuestion;
 
-  return f'', ok', counter;
+  return f'_out, ok_out, counter;
 }
+
 
 
 method correct_apt_ratio(f:Map_Map_T<int, bool, bool>, x:real, y:real, ghost counter_in:nat) returns (r:bool, ghost counter:nat)
@@ -96,6 +98,7 @@ method correct_apt_ratio(f:Map_Map_T<int, bool, bool>, x:real, y:real, ghost cou
   while (!f'Empty)
     decreases f'.Cardinality()
     invariant in_universe_Map_Map_T(f', f)
+    invariant f'Empty == (f'.Cardinality() == 0)
     invariant numTotal == (f.Cardinality() - f'.Cardinality())
     invariant numApt == |(set aptCand:candidate | aptCand in (f.Keys() - f'.Keys()) && f.Model()[aptCand] :: aptCand)|
   {
@@ -118,14 +121,14 @@ method correct_apt_ratio(f:Map_Map_T<int, bool, bool>, x:real, y:real, ghost cou
     f'Empty, counter := f'.Empty(counter);
 
   }
-  assume f'.Cardinality() == 0 && f'.Keys()=={};
   assert numTotal == f.Cardinality();
-    assume false;
-
+  identity_substraction_lemma(f.Keys(), f'.Keys());
   assert numApt == |(set aptCand:candidate | aptCand in (f.Keys()) && f.Model()[aptCand] :: aptCand)|;
   var aptRatio:real := (numApt as real) / (numTotal as real);
-  return (aptRatio <= x || y <= aptRatio), counter;   // ???
+  return (aptRatio <= x || y <= aptRatio), counter;
 }
+
+
 
 method correct_private_ratio(f:Map_Map_T<int, bool, bool>, P:Set<int>, a:real, b:real, ghost counter_in:nat) returns (r:bool, ghost counter:nat)
   requires f.Valid()
@@ -135,7 +138,7 @@ method correct_private_ratio(f:Map_Map_T<int, bool, bool>, P:Set<int>, a:real, b
   requires forall c:candidate | c in f.Keys() :: (P.Model() <= c.Keys)
   requires f.Cardinality() != 0
   ensures r == forall p:int | p in P.Model() ::
-                 (
+                (
                   var privateRatio:real := (|(set isPrivate:candidate | isPrivate in f.Keys() && isPrivate[p] :: isPrivate)| as real) / (f.Cardinality() as real);
                   a <= privateRatio <= b
                 )
@@ -144,65 +147,200 @@ method correct_private_ratio(f:Map_Map_T<int, bool, bool>, P:Set<int>, a:real, b
 
   r := true;
   var P':Set<int>; P', counter := P.Copy(counter);
-  var P'Empty:bool; P'Empty, counter := P.Empty(counter);
+  var P'Empty:bool; P'Empty, counter := P'.Empty(counter);
   while (!P'Empty)
     decreases P'.Cardinality()
     invariant in_universe_Set(P', P)
+    invariant P'Empty == (P'.Cardinality() == 0)
+    invariant r == forall p:int | p in (P.Model() - P'.Model()) ::
+                (
+                  var privateRatio:real := (|(set isPrivate:candidate | isPrivate in f.Keys() && isPrivate[p] :: isPrivate)| as real) / (f.Cardinality() as real);
+                  a <= privateRatio <= b
+                )
   {
-    var p:int; p, counter := P.Pick(counter);
-
-    var f':Map_Map_T<int, bool, bool>; f', counter := f.Copy(counter);
-    var f'Empty:bool; f'Empty, counter := f'.Empty(counter);
-    var numPriv:int := 0;
-    var numTotal:int := 0;
-    
-    while (!f'Empty)
-      decreases f'.Cardinality()
-      invariant in_universe_Map_Map_T(f', f)
-      invariant numTotal == (f.Cardinality() - f'.Cardinality())
-      invariant numPriv == |(set privCand:candidate | privCand in (f.Keys() - f'.Keys()) && privCand[p] :: privCand)|
-    {
-      ghost var f'prev := f';
-      var cand:Map<int, bool>; cand, counter := f'.PickKey(counter);
-      f', counter := f'.Remove(cand, counter);
-      var isPrivate:bool; isPrivate, counter := cand.Get(p, counter);
-      if (isPrivate) {
-        numPriv := numPriv + 1;
-      }
-
-      assert numPriv == |(set privCand:candidate | privCand in (f.Keys() - f'.Keys()) && privCand[p] :: privCand)| by {
-        assert f'prev.Keys() == (f'.Keys() + {cand.Model()});
-        assert (f.Keys() - (f'.Keys() + {cand.Model()})) == (f.Keys() - f'.Keys() - {cand.Model()});
-        assert if isPrivate then numPriv == |(set privCand:candidate | privCand in (f.Keys() - f'.Keys() - {cand.Model()}) && privCand[p] :: privCand)| + 1
-              else           numPriv == |(set privCand:candidate | privCand in (f.Keys() - f'.Keys() - {cand.Model()}) && privCand[p] :: privCand)|;
-        lemma_card_priv_set_when_remove_element(f.Model(), f.Keys() - f'.Keys(), cand.Model(), p);
-      }
-
-      
-      numTotal := numTotal + 1;
-      f'Empty, counter := f'.Empty(counter);
-    }
-
-    var privateRatio:real := (numPriv as real) / (numTotal as real);
-
-    assert forall p:int | p in P.Model() ::
-          (
-            var privateRatio:real := (|(set isPrivate:candidate | isPrivate in f.Keys() && isPrivate[p] :: isPrivate)| as real) / (f.Cardinality() as real);
-            a <= privateRatio <= b
-          );
-
-    r := r && (a <= privateRatio <= b);
+    r, P', P'Empty, counter := correct_private_ratio_outer_loop(f, P, P', a, b, r, counter);
   }
+  identity_substraction_lemma(P.Model(), P'.Model());
 
   return r, counter;
 }
 
 
-method candidates_with_same_answer<T>(f:Map_Map_T<int, bool, T>, question:int, answer:bool, ghost counter_in:nat) returns (f':Map_Map_T<int, bool, T>, ghost counter:nat)
+method correct_private_ratio_outer_loop(f:Map_Map_T<int, bool, bool>, P:Set<int>, P':Set<int>, a:real, b:real, r:bool, ghost counter_in:nat) returns (r_out:bool, P'_out:Set<int>, P'Empty:bool, ghost counter:nat)
+  requires f.Valid()
+  requires forall c1, c2:candidate |  c1 in f.Keys() && c2 in f.Keys() :: c1.Keys == c2.Keys
+  requires 0.0 <= a <= b <= 1.0
+  requires forall c:candidate | c in f.Keys() :: (P.Model() <= c.Keys)
+  requires f.Cardinality() != 0
+
+  requires in_universe_Set(P', P)
+  requires P'.Cardinality() != 0
+  requires r == forall p:int | p in (P.Model() - P'.Model()) ::
+              (
+                var privateRatio:real := (|(set isPrivate:candidate | isPrivate in f.Keys() && isPrivate[p] :: isPrivate)| as real) / (f.Cardinality() as real);
+                a <= privateRatio <= b
+              )
+  
+  ensures P'_out.Cardinality() < P'.Cardinality()
+  ensures in_universe_Set(P'_out, P)
+  ensures P'Empty == (P'_out.Cardinality() == 0)
+  ensures r_out == forall p:int | p in (P.Model() - P'_out.Model()) ::
+              (
+                var privateRatio:real := (|(set isPrivate:candidate | isPrivate in f.Keys() && isPrivate[p] :: isPrivate)| as real) / (f.Cardinality() as real);
+                a <= privateRatio <= b
+              )
+
+{
+  counter := counter_in;
+  var p:int; p, counter := P'.Pick(counter);
+  
+  P'_out, counter := P'.Remove(p, counter);
+
+  var f':Map_Map_T<int, bool, bool>; f', counter := f.Copy(counter);
+  var numPriv:int := 0;
+  var numTotal:int := 0;
+  var f'Empty:bool; f'Empty, counter := f'.Empty(counter);
+  
+  while (!f'Empty)
+    decreases f'.Cardinality()
+    invariant in_universe_Map_Map_T(f', f)
+    invariant numTotal == (f.Cardinality() - f'.Cardinality())
+    invariant numPriv == |(set privCand:candidate | privCand in (f.Keys() - f'.Keys()) && privCand[p] :: privCand)|
+    invariant f'Empty == (f'.Cardinality() == 0)
+  {
+    f', f'Empty, numTotal, numPriv, counter := correct_private_ratio_inner_loop(f, f', p, numTotal, numPriv, counter);
+  }
+  identity_substraction_lemma(f.Keys(), f'.Keys());
+  var privateRatio:real := (numPriv as real) / (numTotal as real);
+
+  r_out := r && (a <= privateRatio <= b);
+  P'Empty, counter := P'_out.Empty(counter);
+
+
+  assert privateRatio == (|(set isPrivate:candidate | isPrivate in f.Keys() && isPrivate[p] :: isPrivate)| as real) / (f.Cardinality() as real) by {
+    assert (numTotal as real) == (f.Cardinality() as real);
+    assert (numPriv as real) == (|(set isPrivate:candidate | isPrivate in f.Keys() && isPrivate[p] :: isPrivate)| as real);
+  }
+  lemma_private_ratio(f, P, P', P'_out, a, b, r, r_out, p, privateRatio);
+  
+  return r_out, P'_out, P'Empty, counter;
+}
+
+
+method correct_private_ratio_inner_loop(f:Map_Map_T<int, bool, bool>, f':Map_Map_T<int, bool, bool>, p:int, numTotal:int, numPriv:int, ghost counter_in:nat) returns (f'_out:Map_Map_T<int, bool, bool>, f'_Empty:bool, numTotal':int, numPriv':int, ghost counter:nat)
+  requires f.Valid()
+  requires forall c1, c2:candidate |  c1 in f.Keys() && c2 in f.Keys() :: c1.Keys == c2.Keys
+  requires forall c:candidate | c in f.Keys() :: (p in c.Keys)
+  requires f.Cardinality() != 0
+  
+  requires in_universe_Map_Map_T(f', f)
+  requires numTotal == (f.Cardinality() - f'.Cardinality())
+  requires numPriv == |(set privCand:candidate | privCand in (f.Keys() - f'.Keys()) && privCand[p] :: privCand)|
+  
+  ensures f'_out.Cardinality() < f'.Cardinality()
+  
+  ensures in_universe_Map_Map_T(f'_out, f)
+  ensures numTotal' == (f.Cardinality() - f'_out.Cardinality())
+  ensures numPriv' == |(set privCand:candidate | privCand in (f.Keys() - f'_out.Keys()) && privCand[p] :: privCand)|
+  ensures f'_Empty == (f'_out.Cardinality() == 0)
+{
+  counter := counter_in;
+  numPriv' := numPriv;
+
+  var cand:Map<int, bool>; cand, counter := f'.PickKey(counter);
+  f'_out, counter := f'.Remove(cand, counter);
+  var isPrivate:bool; isPrivate, counter := cand.Get(p, counter);
+  if (isPrivate) {
+    numPriv' := numPriv + 1;
+  }
+
+  assert numPriv' == |(set privCand:candidate | privCand in (f.Keys() - f'_out.Keys()) && privCand[p] :: privCand)| by {
+    assert f'.Keys() == (f'_out.Keys() + {cand.Model()});
+    assert (f.Keys() - (f'_out.Keys() + {cand.Model()})) == (f.Keys() -f'_out.Keys() - {cand.Model()});
+    assert if isPrivate then numPriv' == |(set privCand:candidate | privCand in (f.Keys() - f'_out.Keys() - {cand.Model()}) && privCand[p] :: privCand)| + 1
+            else           numPriv' == |(set privCand:candidate | privCand in (f.Keys() - f'_out.Keys() - {cand.Model()}) && privCand[p] :: privCand)|;
+    lemma_card_priv_set_when_remove_element(f.Model(), f.Keys() - f'_out.Keys(), cand.Model(), p);
+  }
+  
+  numTotal' := numTotal + 1;
+  f'_Empty, counter := f'_out.Empty(counter);
+
+  return f'_out, f'_Empty, numTotal', numPriv', counter;
+}
+
+
+
+method candidates_with_same_answer<T>(f:Map_Map_T<int, bool, T>, question:int, answer:bool, ghost counter_in:nat) returns (f_out:Map_Map_T<int, bool, T>, ghost counter:nat)
   requires f.Valid()
   requires forall c1, c2:candidate |  c1 in f.Keys() && c2 in f.Keys() :: c1.Keys == c2.Keys
   requires forall c:candidate |  c in f.Keys() :: question in c
-  ensures f'.Model() == (map c:candidate | c in f.Keys() && c[question] == answer :: f.Model()[c])
+  ensures f_out.Model() == (map c:candidate | c in f.Keys() && c[question] == answer :: f.Model()[c])
+{
+  counter := counter_in;
+
+  var f':Map_Map_T<int, bool, T>; f', counter := f.Copy(counter);
+  f_out, counter := New_Map_Map_T_params(f.Model(), f.UBSize_Keys(), counter_in);
+
+  var f'Empty:bool; f'Empty, counter := f'.Empty(counter);
+  
+  while (!f'Empty)
+    decreases f'.Cardinality()
+    invariant in_universe_Map_Map_T(f', f)
+    invariant in_universe_Map_Map_T(f_out, f)
+    invariant f'Empty == (f'.Cardinality() == 0)
+    invariant f_out.Model() == (map c:candidate | c in (f.Keys() - f'.Keys()) && c[question] == answer :: f.Model()[c])
+  {
+    f', f_out, f'Empty, counter := candidates_with_same_answer_loop(f, f', f_out, question, answer, counter);
+  }
+  identity_substraction_lemma(f.Keys(), f'.Keys());
+
+  return f_out, counter;
+}
+
+
+method candidates_with_same_answer_loop<T>(f:Map_Map_T<int, bool, T>, f':Map_Map_T<int, bool, T>, f'':Map_Map_T<int, bool, T>, question:int, answer:bool, ghost counter_in:nat) returns (f'_out:Map_Map_T<int, bool, T>, f''_out:Map_Map_T<int, bool, T>, f'Empty:bool, ghost counter:nat)
+  requires forall c1, c2:candidate |  c1 in f.Keys() && c2 in f.Keys() :: c1.Keys == c2.Keys
+  requires forall c:candidate |  c in f.Keys() :: question in c
+
+  requires in_universe_Map_Map_T(f', f)
+  requires in_universe_Map_Map_T(f'', f)
+  requires f'.Cardinality() != 0
+  requires f''.Model() == (map c:candidate | c in (f.Keys() - f'.Keys()) && c[question] == answer :: f.Model()[c])
+
+  ensures f'_out.Cardinality() < f'.Cardinality()
+
+  ensures in_universe_Map_Map_T(f'_out, f)
+  ensures in_universe_Map_Map_T(f''_out, f)
+  ensures f'Empty == (f'_out.Cardinality() == 0)
+  
+  ensures f''_out.Model() == (map c:candidate | c in (f.Keys() - f'_out.Keys()) && c[question] == answer :: f.Model()[c])
+{
+  counter := counter_in;
+  var cand:Map<int, bool>; cand, counter := f'.PickKey(counter);
+  f'_out, counter := f'.Remove(cand, counter);
+
+  var cand_answer:bool; cand_answer, counter := cand.Get(question, counter);
+  if (cand_answer == answer) {
+    var f_cand:T; f_cand, counter := f.Get(cand, counter);
+    f''_out, counter := f''.Insert(cand, f_cand, counter);
+
+    assert (forall k | k in f''.Universe().Keys :: f''_out.Universe()[k] == f.Model()[k]);
+    candidates_with_same_answer_lemma_1<T>(f, f',  f'', f'_out, f''_out, cand, question, answer);
+  }
+  else {
+    f''_out, counter := f''.Copy(counter);
+    candidates_with_same_answer_lemma_2(f, f',  f'', f'_out, f''_out, cand, question, answer);
+  }
+
+  f'Empty, counter := f'_out.Empty(counter);
+
+  return f'_out, f''_out, f'Empty, counter;
+}
+
+
+
+// LEMMAS
+
 
 
 lemma lemma_card_apt_set_when_remove_element(f:map<candidate, bool>, cands:set<candidate>, cand:candidate)
@@ -228,6 +366,8 @@ lemma lemma_card_apt_set_when_remove_element(f:map<candidate, bool>, cands:set<c
             (set aptCand:candidate | aptCand in cands && f[aptCand] :: aptCand);
   }
 }
+
+
 lemma lemma_card_priv_set_when_remove_element(f:map<candidate, bool>, cands:set<candidate>, cand:candidate, p:int)
   requires cand in cands
   requires cands <= f.Keys
@@ -252,3 +392,122 @@ lemma lemma_card_priv_set_when_remove_element(f:map<candidate, bool>, cands:set<
             (set privCand:candidate | privCand in cands && privCand[p] :: privCand);
   }
 }
+
+
+
+lemma lemma_private_ratio(f:Map_Map_T<int, bool, bool>, P:Set<int>, P':Set<int>, P'':Set<int>, a:real, b:real, r:bool, r':bool, p:int, privateRatio:real)
+  requires f.Valid()
+  requires forall c1, c2:candidate |  c1 in f.Keys() && c2 in f.Keys() :: c1.Keys == c2.Keys
+  requires 0.0 <= a <= b <= 1.0
+  requires forall c:candidate | c in f.Keys() :: (P.Model() <= c.Keys)
+  requires f.Cardinality() != 0
+
+  requires in_universe_Set(P', P)
+  requires P'.Cardinality() != 0
+  requires r == forall p:int | p in (P.Model() - P'.Model()) ::
+              (
+                var privateRatio:real := (|(set isPrivate:candidate | isPrivate in f.Keys() && isPrivate[p] :: isPrivate)| as real) / (f.Cardinality() as real);
+                a <= privateRatio <= b
+              )
+  
+
+  requires P'.Model() == (P''.Model() + {p})
+  requires p !in P''.Model()
+  requires privateRatio == (|(set isPrivate:candidate | isPrivate in f.Keys() && isPrivate[p] :: isPrivate)| as real) / (f.Cardinality() as real)
+  requires r' == (r && (a <= privateRatio <= b))
+
+  ensures r' == forall p:int | p in (P.Model() - P''.Model()) ::
+              (
+                var privateRatio:real := (|(set isPrivate:candidate | isPrivate in f.Keys() && isPrivate[p] :: isPrivate)| as real) / (f.Cardinality() as real);
+                a <= privateRatio <= b
+              )
+
+{
+  assert r == forall p:int | p in (P.Model() - P'.Model()) ::
+              (
+                var privateRatio:real := (|(set isPrivate:candidate | isPrivate in f.Keys() && isPrivate[p] :: isPrivate)| as real) / (f.Cardinality() as real);
+                a <= privateRatio <= b
+              );
+  assert r' == ((forall p:int | p in (P.Model() - P'.Model()) ::
+              (
+                var privateRatio:real := (|(set isPrivate:candidate | isPrivate in f.Keys() && isPrivate[p] :: isPrivate)| as real) / (f.Cardinality() as real);
+                a <= privateRatio <= b
+              ))
+              &&
+              (a <= privateRatio <= b))
+              ;
+  assert (P.Model() - P''.Model()) == ((P.Model() - P'.Model()) + {p});
+}
+
+
+
+lemma candidates_with_same_answer_lemma_1<T>(f:Map_Map_T<int, bool, T>, f':Map_Map_T<int, bool, T>,  f'':Map_Map_T<int, bool, T>, f'_out:Map_Map_T<int, bool, T>, f''_out:Map_Map_T<int, bool, T>, cand:Map<int, bool>, question:int, answer:bool)
+  requires forall c1, c2:candidate |  c1 in f.Keys() && c2 in f.Keys() :: c1.Keys == c2.Keys
+  requires forall c:candidate |  c in f.Keys() :: question in c
+  requires in_universe_Map_Map_T(f', f)
+  requires in_universe_Map_Map_T(f'', f)
+  requires f'.Cardinality() != 0
+  requires f''.Model() == (map c:candidate | c in (f.Keys() - f'.Keys()) && c[question] == answer :: f.Model()[c])
+
+  requires f'_out.Keys() == f'.Keys() - {cand.Model()}
+  requires cand.Model() in f'.Model()
+  requires cand.Model()[question] == answer
+  requires f''_out.Model() == f''.Model()[cand.Model() := f.Model()[cand.Model()]]
+
+  ensures f''_out.Model() == (map c:candidate | c in (f.Keys() - f'_out.Keys()) && c[question] == answer :: f.Model()[c])
+{
+  assert f''_out.Model() == (map c:candidate | c in (f.Keys() - f'.Keys()) && c[question] == answer :: f.Model()[c])[cand.Model() := f.Model()[cand.Model()]];
+  candidates_with_same_answer_lemma_1_aux(f, f', cand, question, answer);
+  assert f''_out.Model() == (map c:candidate | c in (f.Keys() - f'.Keys() + {cand.Model()}) && c[question] == answer :: f.Model()[c]);
+
+  assert f'_out.Keys() == f'.Keys() - {cand.Model()};
+  assert (f.Keys() - f'.Keys() + {cand.Model()}) == (f.Keys() - f'_out.Keys());
+}
+
+
+lemma candidates_with_same_answer_lemma_2<T>(f:Map_Map_T<int, bool, T>, f':Map_Map_T<int, bool, T>,  f'':Map_Map_T<int, bool, T>, f'_out:Map_Map_T<int, bool, T>, f''_out:Map_Map_T<int, bool, T>, cand:Map<int, bool>, question:int, answer:bool)
+  requires forall c1, c2:candidate |  c1 in f.Keys() && c2 in f.Keys() :: c1.Keys == c2.Keys
+  requires forall c:candidate |  c in f.Keys() :: question in c
+  requires in_universe_Map_Map_T(f', f)
+  requires in_universe_Map_Map_T(f'', f)
+  requires f'.Cardinality() != 0
+  requires f''.Model() == (map c:candidate | c in (f.Keys() - f'.Keys()) && c[question] == answer :: f.Model()[c])
+
+  requires f'_out.Keys() == f'.Keys() - {cand.Model()}
+  requires cand.Model() in f'.Model()
+  requires cand.Model()[question] != answer
+  requires f''_out.Model() == f''.Model()
+
+  ensures f''_out.Model() == (map c:candidate | c in (f.Keys() - f'_out.Keys()) && c[question] == answer :: f.Model()[c])
+{
+  assert f''_out.Model() == f''.Model();
+  assert f''_out.Model() == (map c:candidate | c in (f.Keys() - f'.Keys()) && c[question] == answer :: f.Model()[c]);
+  candidates_with_same_answer_lemma_2_aux(f, f'_out, cand, question, answer);
+  assert f''_out.Model() == (map c:candidate | c in (f.Keys() - f'_out.Keys() - {cand.Model()}) && c[question] == answer :: f.Model()[c]);
+  assert forall c:candidate | c in (f.Keys() - f'_out.Keys() - {cand.Model()}) && c[question] == answer :: c !in {cand.Model()};
+  assert forall c:candidate | c in (f.Keys() - f'_out.Keys() - {cand.Model()}) && c[question] == answer :: c in (f.Keys() - f'_out.Keys());
+
+  assert (map c:candidate | c in (f.Keys() - f'_out.Keys() - {cand.Model()}) && c[question] == answer :: f.Model()[c]) ==
+          (map c:candidate | c in (f.Keys() - f'_out.Keys()) && c[question] == answer :: f.Model()[c]);
+}
+
+
+lemma candidates_with_same_answer_lemma_1_aux<T>(f:Map_Map_T<int, bool, T>, f':Map_Map_T<int, bool, T>, cand:Map<int, bool>, question:int, answer:bool)
+  requires forall c:candidate |  c in f.Keys() :: question in c
+  requires cand.Model() in f.Model()
+  requires cand.Model()[question] == answer
+
+  ensures 
+          (map c:candidate | c in (f.Keys() - f'.Keys()) && c[question] == answer :: f.Model()[c])[cand.Model() := f.Model()[cand.Model()]]
+          ==
+          (map c:candidate | c in (f.Keys() - f'.Keys() + {cand.Model()}) && c[question] == answer :: f.Model()[c])
+{}
+
+lemma candidates_with_same_answer_lemma_2_aux<T>(f:Map_Map_T<int, bool, T>, f'_out:Map_Map_T<int, bool, T>, cand:Map<int, bool>, question:int, answer:bool)
+  requires forall c:candidate |  c in f.Keys() :: question in c
+  requires cand.Model() in f.Model()
+  requires cand.Model()[question] != answer
+
+  ensures (map c:candidate | c in (f.Keys() - f'_out.Keys() - {cand.Model()}) && c[question] == answer :: f.Model()[c]) ==
+          (map c:candidate | c in (f.Keys() - f'_out.Keys()) && c[question] == answer :: f.Model()[c])
+{}
